Add bounded buffer queue refinement proof

Lib/KVMap.v
@@ -1,4 +1,5 @@
 From Coq Require Import
+  Arith
   List.
 From FunProofs.Lib Require Import
   EqDec
@@ -10,14 +11,14 @@ Section KVMap.
 
   Definition kvmap := key -> value.
 
-  Definition initmap (d : value) : kvmap := fun _ => d.
-  Definition getvar (k : key) (m : kvmap) : value := m k.
-  Definition setvar (kv : key * value) (m : kvmap) : kvmap :=
-    fun k' => if fst kv == k' then snd kv else getvar k' m.
-  Definition setvars (kvs : list (key * value)) (m : kvmap) : kvmap :=
-    fold_right setvar m kvs.
-  Definition buildmap (d : value) (kvs : list (key * value)) : kvmap :=
-    setvars kvs (initmap d).
+  Definition kvinit (d : value) : kvmap := fun _ => d.
+  Definition kvget (k : key) (m : kvmap) : value := m k.
+  Definition kvset (kv : key * value) (m : kvmap) : kvmap :=
+    fun k' => if fst kv == k' then snd kv else kvget k' m.
+  Definition kvsets (kvs : list (key * value)) (m : kvmap) : kvmap :=
+    fold_right kvset m kvs.
+  Definition kvbuild (d : value) (kvs : list (key * value)) : kvmap :=
+    kvsets kvs (kvinit d).
 End KVMap.
 
 Arguments kvmap _ _ : clear implicits.
@@ -25,35 +26,127 @@ Arguments kvmap _ _ : clear implicits.
 Declare Scope kvmap.
 Delimit Scope kvmap with kvmap.
 Notation "k |-> v" := (k, v) (at level 10) : kvmap.
-Notation "m @ k" := (getvar k m) (at level 20) : kvmap.
-Notation "m ! k" := (setvar k m) (at level 20) : kvmap.
+Notation "m @ k" := (kvget k m) (at level 20) : kvmap.
+Notation "m ! k" := (kvset k m) (at level 20) : kvmap.
 Notation "{ kv1 , .. , kvn } [ d ]" :=
-  (buildmap d (cons kv1%kvmap .. (cons kvn%kvmap nil) ..)) : kvmap.
+  (kvbuild d (cons kv1%kvmap .. (cons kvn%kvmap nil) ..)) : kvmap.
 
 Section KVMap.
   Open Scope kvmap.
   Context {key value : Type} `{EqDec key}.
 
-  Lemma get_set_same : forall k v (m : kvmap key value),
-    m ! (k, v) @ k = v.
+  Lemma kvget_init : forall (k : key) (d : value), kvinit d @ k = d.
+  Proof. auto. Qed.
+
+  Lemma kvget_set_same : forall k v (m : kvmap key value),
+    m ! (k |-> v) @ k = v.
   Proof.
-    unfold getvar, setvar; intros; cbn; rewrite eq_dec_true; auto.
+    unfold kvget, kvset; intros; cbn; rewrite eq_dec_true; auto.
   Qed.
 
-  Lemma get_set_other : forall k v' v (m : kvmap key value),
-    k <> v' -> m ! (k, v) @ v' = m @ v'.
+  Lemma kvget_set_other : forall k v' v (m : kvmap key value),
+    k <> v' -> m ! (k |-> v) @ v' = m @ v'.
   Proof.
-    unfold getvar, setvar; intros; cbn; rewrite eq_dec_false; auto.
+    unfold kvget, kvset; intros; cbn; rewrite eq_dec_false; auto.
   Qed.
 
-  Lemma setvars_correct : forall kvs (m : kvmap key value) k v,
-    NoDup (map fst kvs) -> In (k, v) kvs ->
-    setvars kvs m @ k = v.
+  Lemma kvsets_correct : forall kvs (m : kvmap key value) k v,
+    NoDup (map fst kvs) -> In (k |-> v) kvs ->
+    kvsets kvs m @ k = v.
   Proof.
-    induction kvs as [| kv' kvs]; cbn -[getvar]; intros * Huniq Hin;
-      inv Huniq; intuition (subst; auto using get_set_same).
-    destruct kv'; fold (setvars kvs m); rewrite get_set_other; auto.
+    induction kvs as [| kv' kvs]; cbn -[kvget]; intros * Huniq Hin;
+      inv Huniq; intuition (subst; auto using kvget_set_same).
+    destruct kv'; fold (kvsets kvs m); rewrite kvget_set_other; auto.
     intros ->; prename (_ -> False) into Hnin; apply Hnin.
     cbn; rewrite in_map_iff; repeat esplit; eauto; auto.
   Qed.
 End KVMap.
+
+Section Array.
+  Context {value : Type} {sz : nat}.
+
+  Definition array (sz : nat) := kvmap nat (option value).
+
+  Definition arrayinit : array sz := kvinit None.
+  Definition arrayget (k : nat) (a : array sz) : option value :=
+    if k <? sz then kvget k a else None.
+  Definition arrayset (kv : nat * value) (a : array sz) : option (array sz) :=
+    if fst kv <? sz then Some (kvset (fst kv, Some (snd kv)) a) else None.
+  Definition arraysets (kvs : list (nat * value)) (a : array sz) : option (array sz) :=
+    fold_right
+      (fun kv a => match a with Some a => arrayset kv a | None => None end)
+      (Some a)
+      kvs.
+  Definition arraybuild (kvs : list (nat * value)) : option (array sz) :=
+    arraysets kvs arrayinit.
+End Array.
+
+Arguments array _ : clear implicits.
+
+Declare Scope array.
+Delimit Scope array with array.
+Notation "k |-> v" := (k, v) (at level 10) : array.
+Notation "m @ k" := (arrayget k m) (at level 20) : array.
+Notation "m ! k" := (arrayset k m) (at level 20) : array.
+Notation "{ kv1 , .. , kvn } [ d ]" :=
+  (arraybuild d (cons kv1%array .. (cons kvn%array nil) ..)) : array.
+
+Section Array.
+  Open Scope array.
+  Context {value : Type} {sz : nat}.
+
+  Lemma arrayget_init : forall k, (@arrayinit value sz) @ k = None.
+  Proof. unfold arrayget; intros; now destruct (_ <? _). Qed.
+
+  Lemma arrayget_set_same : forall k v (a a' : array value sz),
+    a ! (k |-> v) = Some a' ->
+    a' @ k = Some v.
+  Proof.
+    unfold arrayget, arrayset; cbn [fst]; intros * Hset.
+    cases Hset; simplify; now rewrite kvget_set_same.
+  Qed.
+
+  Lemma arrayget_set_other : forall k v' v (a a' : array value sz),
+    k <> v' ->
+    a ! (k |-> v) = Some a' ->
+    a' @ v' = a @ v'.
+  Proof.
+    unfold arrayget, arrayset; cbn [fst]; intros * ? Hset.
+    cases Hset; simplify; now rewrite kvget_set_other.
+  Qed.
+
+  Lemma arrayget_oob : forall (a : array value sz) (idx : nat),
+    sz <= idx ->
+    a @ idx = None.
+  Proof.
+    unfold arrayget; intros * Hoob.
+    apply Nat.leb_le in Hoob.
+    rewrite Nat.ltb_antisym, Hoob; auto.
+  Qed.
+
+  Lemma arrayget_in : forall (a : array value sz) (idx : nat) v,
+    a @ idx = Some v ->
+    idx < sz.
+  Proof.
+    unfold arrayget; intros * Hget.
+    cases Hget; apply Nat.leb_le; auto.
+  Qed.
+
+  Lemma arrayset_oob : forall (a : array value sz) (idx : nat) v,
+    sz <= idx <-> a ! (idx |-> v) = None.
+  Proof.
+    unfold arrayset; split; cbn [fst]; [intros Hoob | intros Hset].
+    - apply Nat.leb_le in Hoob.
+      rewrite Nat.ltb_antisym, Hoob; auto.
+    - apply Nat.leb_le; rewrite Nat.leb_antisym.
+      cases Hset; auto.
+  Qed.
+
+  Corollary arrayset_in : forall (a a' : array value sz) (idx : nat) v,
+    a ! (idx |-> v) = Some a' ->
+    idx < sz.
+  Proof.
+    intros * Hset.
+    now rewrite Nat.lt_nge, arrayset_oob, Hset.
+  Qed.
+End Array.
