BBQ.v
@@ -1,0 +1,170 @@
+(*
+ * Bounded Buffer Queue implementation using an "array" (finite map).
+ *)
+
+From Coq Require Import
+  Arith
+  Lia
+  List.
+From FunProofs.Lib Require Import
+  KVMap
+  Util.
+Import EqDecNotations.
+
+Open Scope array.
+
+Section BBQ.
+  Record bbq {A} {maxsize : nat} := mkBBQ {
+    buf: array A maxsize;
+    head: nat;
+    size: nat;
+  }.
+  Global Arguments bbq _ _ : clear implicits.
+
+  Inductive BBQError := BBQFull | BBQEmpty | BBQOOB.
+
+  Notation Res A := (A + BBQError)%type.
+  Notation Ok := (@inl _ BBQError).
+  Notation Err := (@inr _ BBQError).
+
+  Definition bbq_init A sz : bbq A sz := mkBBQ A sz arrayinit 0 0.
+
+  Definition bbq_empty {A sz} (q : bbq A sz) : bool := q.(size) ==? 0.
+  Definition bbq_full {A sz} (q : bbq A sz) : bool := sz ==? q.(size).
+
+  Definition bbq_enqueue {A sz} (q : bbq A sz) (v : A) : Res (bbq A sz) :=
+    if bbq_full q then Err BBQFull
+    else
+      let idx := (q.(head) + q.(size)) mod sz in
+      let buf' := q.(buf) ! (idx |-> v) in
+      match buf' with
+      | Some buf' =>
+        Ok {|
+          buf := buf';
+          head := q.(head);
+          size := q.(size) + 1;
+        |}
+      | None => Err BBQOOB (* Impossible *)
+      end.
+
+  Definition bbq_dequeue {A sz} (q : bbq A sz) : Res (bbq A sz * A) :=
+    if bbq_empty q then Err BBQEmpty
+    else
+      let v := q.(buf) @ q.(head) in
+      match v with
+      | Some v =>
+        Ok ({|
+          buf := q.(buf);
+          head := (q.(head) + 1) mod sz;
+          size := q.(size) - 1;
+        |}, v)
+      | None => Err BBQOOB (* Impossible *)
+      end.
+
+  Record bbq_bounds {A sz} (q : bbq A sz) : Prop := {
+    bbq_size_bounds : q.(size) <= sz;
+    bbq_head_bounds : q.(head) < sz;
+  }.
+
+  Lemma bbq_init_bounds {A sz} : 0 < sz -> bbq_bounds (bbq_init A sz).
+  Proof. constructor; cbn; lia. Qed.
+
+  Lemma bbq_enqueue_bounds {A sz} : forall (q q' : bbq A sz) v,
+    0 < sz -> bbq_bounds q ->
+    bbq_enqueue q v = Ok q' ->
+    bbq_bounds q'.
+  Proof.
+    unfold bbq_enqueue, bbq_full, eqb; intros * Hsz Hbounds Hq.
+    cases *; inv Hbounds; simplify.
+    constructor; cbn; lia.
+  Qed.
+
+  Lemma bbq_dequeue_bounds {A sz} : forall (q q' : bbq A sz) v,
+    0 < sz -> bbq_bounds q ->
+    bbq_dequeue q = Ok (q', v) ->
+    bbq_bounds q'.
+  Proof.
+    unfold bbq_dequeue; intros * Hsz Hbounds Hq.
+    cases Hq; inv Hbounds; simplify.
+    pose proof (Nat.mod_upper_bound (q.(head) + 1) sz).
+    constructor; cbn; lia.
+  Qed.
+
+  Record bbq_list_R {A sz} (q : bbq A sz) (lq : list A) : Prop := {
+    bbq_list_bounds : bbq_bounds q;
+    bbq_list_length : length lq = q.(size);
+    bbq_list_nth : forall n, n < q.(size) ->
+      q.(buf) @ ((q.(head) + n) mod sz) = nth_error lq n;
+  }.
+
+  Lemma bbq_list_refine_init {A sz} : 0 < sz -> bbq_list_R (bbq_init A sz) nil.
+  Proof.
+    constructor; cbn; intros; auto using bbq_init_bounds.
+    now rewrite arrayget_init, nth_error_nil.
+  Qed.
+
+  Lemma bbq_list_refine_enqueue {A sz} : forall (q : bbq A sz) lq v,
+    0 < sz ->
+    bbq_list_R q lq ->
+    match bbq_enqueue q v with
+    | inl q' => bbq_list_R q' (lq @@ v)
+    | inr BBQFull => length lq = sz
+    | _ => False
+    end.
+  Proof.
+    intros * Hsz HR; inv HR.
+    remember (bbq_enqueue q v) as res eqn:Hq.
+    pose proof Hq; unfold bbq_enqueue, bbq_full, eqb in Hq.
+    cases *; simplify; auto.
+    - constructor; cbn; eauto using bbq_enqueue_bounds; [rewrite app_length; auto |].
+      inv bbq_list_bounds0.
+      intros n' Hlt.
+      assert (n' < q.(size) \/ n' = q.(size)) as [|] by lia; subst.
+      + specialize (bbq_list_nth0 n' ltac:(auto)).
+        rewrite nth_error_app1, <- bbq_list_nth0 by lia.
+        eapply arrayget_set_other; [intros Heq | eauto].
+        assert (~((q.(head) + q.(size)) < sz)).
+        { intros ?; rewrite !Nat.mod_small in Heq; lia. }
+        rewrite Nat.mod_eq, div_range with (n := 1) in Heq by lia.
+        assert (~(q.(head) + n') < sz).
+        { intros ?; rewrite !Nat.mod_small in Heq; lia. }
+        rewrite Nat.mod_eq, div_range with (n := 1) in Heq by lia.
+        lia.
+      + erewrite arrayget_set_same; eauto.
+        rewrite <- bbq_list_length0, nth_error_app2, Nat.sub_diag; auto.
+    - pose proof (Nat.mod_upper_bound (q.(head) + q.(size)) sz).
+      apply arrayset_oob in Hq_case0; lia.
+  Qed.
+
+  Lemma bbq_list_refine_dequeue {A sz} : forall (q : bbq A sz) lq,
+    0 < sz ->
+    bbq_list_R q lq ->
+    match bbq_dequeue q with
+    | inl (q', v) =>
+      match lq with
+      | v' :: lq' => v = v' /\ bbq_list_R q' lq'
+      | nil => False
+      end
+    | inr BBQEmpty => length lq = 0
+    | _ => False
+    end.
+  Proof.
+    intros * Hsz HR; inv HR.
+    remember (bbq_dequeue q) as res eqn:Hq.
+    pose proof Hq; unfold bbq_dequeue, bbq_empty, eqb in Hq.
+    cases *; simplify; auto.
+    - destruct lq; cbn in bbq_list_length0; [lia | split].
+      + inv bbq_list_bounds0.
+        specialize (bbq_list_nth0 0 ltac:(lia)).
+        rewrite Nat.add_0_r, Nat.mod_small in bbq_list_nth0 by lia; simplify; auto.
+      + constructor; cbn; eauto using bbq_dequeue_bounds; [lia |].
+        inv bbq_list_bounds0.
+        intros n' Hlt.
+        specialize (bbq_list_nth0 (1 + n') ltac:(lia)).
+        now rewrite Nat.add_assoc, Nat.add_mod, (Nat.mod_small n') in bbq_list_nth0 by lia.
+    - inv bbq_list_bounds0.
+      specialize (bbq_list_nth0 0 ltac:(lia)).
+      rewrite Nat.add_0_r, Nat.mod_small in bbq_list_nth0 by lia.
+      destruct lq; cbn in *; congruence.
+  Qed.
+End BBQ.
